tests/test_used_axioms.v
@@ -4,7 +4,8 @@ From D.Dot.examples Require examples fromPDotMutualRecSem.
 
 Print Assumptions type_soundness.
 Print Assumptions path_normalization.
-Print Assumptions examples.examples.vSafe.
+Print Assumptions examples.examples.miniVSafe.
+Print Assumptions examples.examples.posModVSafe.
 Print Assumptions fromPDotMutualRecSem.pcoreSafe.
 
 From D.Dot.examples Require list.
